% Files using this must be two subfolders
% deep. Adjust the number of ../ for the
% depth of the file.
\input{preamble.tex}

% Put class number, class name, and professor 
% name.
% Use only in case of emergency, this
% should be covered by the preamble.
% \renewcommand\classname{}

% Put the assignment name with \S if 
% necessary for the section and the question 
% numbers.
\renewcommand\assignment{Homework Set VI, Due Friday, February 17, 2023: \S 3.2 \# 76, 86 \S 3.3 \# 134, 138, 146}

\begin{document}
    % Templates
    \iffalse
    % Use these for equations.
    \begin{equation*}
        \begin{gathered}
            Equations go here.
        \end{gathered}
    \end{equation*}

    % Use this if a line of math is too long.
    \resizebox{\hsize}{!}{$Long equation goes here$}

    % Use these for multiple columns.
    \begin{multicol*}{# of columns}
        % Remove the * if you want the columns to be balanced.
    \end{multicol*}

    % Use this to add a horizontal line.
    \horizontal

    \fi

    % Begin homework here.
    %%%%%%%%%%%%%%%%%%%%%%

    \paragraph*{76.} 
    $\int\sin^7(2x)\cos(2x)dx$
    \\
    \begin{mdframed}
        \begin{equation*}
            \begin{gathered}
                \text{Let} \quad u = \sin(2x) \quad \frac{du}{2} = \cos(2x)dx    \\
                \Rightarrow \frac{1}{2} \int u^7du              
                = \frac{1}{2}\left(\frac{u^8}{8}\right) + C     
                = \boxed{\frac{\sin^8(2x)}{16} + C}
            \end{gathered}
        \end{equation*}
    \end{mdframed}

    \paragraph*{86.}
    $\int \sqrt{\sin x}\cos^3 x dx$
    \\
    \begin{mdframed}
        \begin{equation*}
            \begin{gathered}      
                \int \sqrt{\sin x}(1-\sin^2 x )\cos x dx
                = \int (\sqrt{\sin x} - \sin^{5/2})\cos x dx                        \\
                \text{Let} \quad u = \sin x \quad du = \cos x dx                    \\
                \Rightarrow \int \left(\sqrt{u} - u^{5/2}\right)du
                = \frac{2u^{3/2}}{3} - \frac{2u^{7/2}}{7} + C
                = \boxed{\frac{2(\sin x)^{3/2}}{3} - \frac{2(\sin x)^{7/2}}{7} + C}
            \end{gathered}
        \end{equation*}
    \end{mdframed}

    \paragraph*{134.}
    $\int \frac{dx}{\sqrt{4-x^2}}$
    \\
    \begin{mdframed}
        \begin{equation*}
            \begin{gathered}
                \text{Using} \quad a^2 - u^2 \Rightarrow  
                u = a\sin\theta; \quad x = 2\sin\theta 
                \quad dx = 2\cos\theta d\theta                                      \\
                \Rightarrow\int \frac{2\cos\theta d \theta}{\sqrt{4-4\sin^2\theta}}    
                \int \frac{2\cos\theta d \theta}{\sqrt{4(1-\sin^2\theta)}}
                = \int \frac{\cos\theta d \theta}{\sqrt{1-\sin^2\theta}}    
                = \int \frac{\cos\theta d \theta}{\sqrt{\cos^2\theta}}      
                = \int \frac{\cos\theta d \theta}{\cos\theta} = \int d\theta        \\
                = \theta + C = \boxed{\sin^{-1}\left(\frac{x}{2}\right) + C} 
            \end{gathered}
        \end{equation*}    
    \end{mdframed}

    \paragraph*{138.}
    $\int \frac{x^{2}dx}{\sqrt{1-x^2}}$
    \\
    \begin{mdframed}
        \begin{equation*}
            \begin{gathered}
                \text{Using} \quad a^2 - u^2 \Rightarrow    
                u = a\sin\theta; \quad x = \sin\theta 
                \quad dx = \cos\theta d \theta                  \\
                \int \frac{\sin^2\theta\cos\theta d \theta}
                {\sqrt{1 - \sin^2\theta}}
                = \int \frac{\sin^2\theta\cos\theta d \theta}
                {\sqrt{\cos^2\theta}} 
                = \int \frac{\sin^2\theta\cos\theta d \theta}
                {\cos\theta}
                = \int \sin^2\theta d \theta \Rightarrow
                \int \frac{1-\cos 2\theta}{2}d\theta            \\
                = \frac{2\theta - \sin 2\theta}{4} + C 
                = \boxed{\frac{2\sin^{-1}(x) - \sin(2\sin^{-1}(x))}{4} + C}
            \end{gathered}
        \end{equation*}
    \end{mdframed}

    \paragraph*{146.}
    $\frac{dx}{(1+x^2)^{3/2}}$
    \\
    \begin{mdframed}
        \begin{equation*}
            \begin{gathered}
                \text{Using} \quad a^2 + u^2 \Rightarrow
                u = a\tan\theta; \quad x = \tan\theta \quad dx 
                = \sec^2\theta d \theta                     \\
                \int \frac{\sec^2\theta d \theta}
                {(1+\tan^2\theta)^{3/2}}
                = \int \frac{\sec^2\theta d \theta} 
                {(\sec^2\theta)^{3/2}}
                = \int \frac{\sec^2\theta d \theta}
                {\sec^3\theta}
                = \int \sec^{-1}\theta d \theta
                = \int \cos\theta d \theta                   \\
                = \sin\theta + C = \boxed{\sin(\tan^{-1}(x)) + C}      
            \end{gathered}
        \end{equation*}
    \end{mdframed}
\end{document}